fin de l'ajout de map2 dans FMapList
git-svn-id: svn://scm.gforge.inria.fr/svnroot/coq-contribs/trunk@264 0cf17b13-060f-0410-b1b1-c666bec9822a

FMapList.v
@@ -24,6 +24,10 @@ Unset Strict Implicit.
 Notation "[]" := nil (at level 0).
 Arguments Scope list [type_scope].
 
+Ltac absurd_hyp h := 
+  let T := type of h in 
+  absurd T.
+
 Module Raw (X:OrderedType).
   Module MX := OrderedTypeFacts X.
 
@@ -34,149 +38,166 @@ Module Raw (X:OrderedType).
 
   Variable elt : Set.
 
-  Definition eq_key (p p':key*elt) := X.eq (fst p) (fst p').
-  Definition eq_key_elt (p p':key*elt) := 
+  Definition eqk (p p':key*elt) := X.eq (fst p) (fst p').
+  Definition eqke (p p':key*elt) := 
           X.eq (fst p) (fst p') /\ (snd p) = (snd p').
+  Definition ltk (p p':key*elt) := X.lt (fst p) (fst p').
 
-  Definition lt_key (p p':key*elt) := X.lt (fst p) (fst p').
+  Hint Unfold eqk eqke ltk.
+  Hint Extern 2 (eqke ?a ?b) => split.
 
-  Definition MapsTo (k:key)(e:elt):= InList eq_key_elt (k,e).
-  Definition In k m := exists e:elt, MapsTo k e m.
-  Definition Empty m := forall (a : key)(e:elt) , ~ MapsTo a e m.
+  Ltac simpl_eqke :=
+    match goal with
+    	H:(eqke _ _) |- _ => 
+          let x:= fresh "eqk" in 
+	  let y := fresh "eqe" in (destruct H as (x,y); simpl in y; simpl in x)
+    end.
 
-  Lemma InList_eq_key_el_eq_key : 
-      forall x m, InList eq_key_elt x m -> InList eq_key x m.
-      induction m; simpl; inversion_clear 1; auto.
-      unfold eq_key, eq_key_elt in *; intuition.
+  Ltac sintuition := try simpl_eqke; intuition.
+
+  (* eqk, eqke are equalities, ltk is a strict order *)
+ 
+  Lemma eqk_refl : forall e, eqk e e.
+    auto.
+  Qed.
+
+  Lemma eqke_refl : forall e, eqke e e.
+    auto.
+  Qed.
+
+  Lemma eqk_sym : forall e e', eqk e e' -> eqk e' e.
+    auto.
+  Qed.
+
+  Lemma eqke_sym : forall e e', eqke e e' -> eqke e' e.
+    intros; sintuition.
+  Qed.
+
+  Lemma eqk_trans : forall e e' e'', eqk e e' -> eqk e' e'' -> eqk e e''.
+    eauto. 
+  Qed.
+
+  Lemma eqke_trans : forall e e' e'', eqke e e' -> eqke e' e'' -> eqke e e''.
+    unfold eqke; intuition eauto; congruence.
+  Qed.
+
+  Hint Resolve eqk_trans eqke_trans eqk_sym eqke_sym eqk_refl eqke_refl.
+
+  Lemma ltk_trans : forall e e' e'', ltk e e' -> ltk e' e'' -> ltk e e''.
+     eauto.
+  Qed.
+
+  Lemma ltk_not_eqk : forall e e', ltk e e' -> ~ eqk e e'.
+    unfold eqk, ltk; auto. (* Hint Unfold devrait rendre ce unfold inutile ? *)
+  Qed.  
+
+   Lemma eqk_not_ltk : forall x x', eqk x x' -> ~ltk x x'.
+     unfold eqk, ltk; auto.
+   Qed.
+   Hint Resolve ltk_not_eqk eqk_not_ltk. 
+
+   Lemma ltk_eqk : forall e e' e'', ltk e e' -> eqk e' e'' -> ltk e e''.
+      eauto.
+   Qed.
+   Hint Resolve ltk_eqk.
+
+   Hint Resolve MX.eq_lt MX.lt_eq.
+
+   Lemma eqk_ltk : forall e e' e'', ltk e e'' -> eqk e e' -> ltk e' e''.
+      intros (k,e) (k',e') (k'',e'').
+      unfold ltk, eqk; eauto.
+   Qed.
+   Hint Resolve eqk_ltk.
+
+   (* eqke is a stricter equality than eqk *)
+ 
+   Lemma eqke_eqk : forall x x', eqke x x' -> eqk x x'.
+     unfold eqk, eqke; intuition.
+   Qed.
+   Hint Resolve eqke_eqk.
+
+  (* ltk ignore the second components *)
+
+   Lemma ltk_right_r : forall x k e e', ltk x (k,e) -> ltk x (k,e').
+      auto.
     Qed.
-      
-    Hint Unfold MapsTo eq_key_elt eq_key lt_key In.
-    Hint Constructors InList.
-    Hint Resolve InList_eq_key_el_eq_key.
+    Hint Resolve ltk_right_r.
+
+    Lemma ltk_right_l : forall x k e e', ltk (k,e) x -> ltk (k,e') x.
+      auto.
+    Qed.
+    Hint Resolve ltk_right_l.
+
+
+  Definition MapsTo (k:key)(e:elt):= InList eqke (k,e).
+  Definition In k m := exists e:elt, MapsTo k e m.
+
+  Hint Unfold MapsTo In.
+
+  Lemma InList_eqke_eqk : 
+     forall x m, InList eqke x m -> InList eqk x m.
+  Proof.
+    induction 1; sintuition.
+  Qed.
+  Hint Resolve InList_eqke_eqk.
+
+  (* An alternative formulation for [In k l] is [exists e, InList eqk (k,e) l] *)
+
+  Lemma InList_eqk_In : forall k e l, InList eqk (k,e) l -> In k l.
+  Proof.
+     induction 1.
+     destruct y.
+     exists e0.
+     eauto.
+     induction IHInList.
+     exists x;eauto.
+  Qed.
+  Hint Resolve InList_eqk_In.
+
+  Lemma In_InList_eqk : forall k e l, In k l -> InList eqk (k,e) l.
+  Proof.
+     induction 1.
+     induction H; simpl; sintuition.
+  Qed.
+  Hint Resolve In_InList_eqk.
+
+  Lemma altern_In : forall k l, In k l <-> exists e:elt, InList eqk (k,e) l.
+  Proof.
+   split.
+   destruct 1. 
+   exists x; auto. 
+   intros (x,H); eauto.
+  Qed.
+
+(*
+    (* could also be proved as a corollary of previous lemma *)
+    Lemma InList_In : forall k e l, InList eqke (k,e) l -> In k l.
+      intros k e l H. exists e;auto.
+    Qed.
+    Hint Resolve InList_In.
+*)
 
     Lemma notin_empty : forall k, ~ In k [].
       intros k abs.
       inversion abs.
       inversion H.
     Qed.
-
     Hint Resolve notin_empty.
 
-    Hint Extern 2 (eq_key_elt ?a ?b) => split.
 
-    Ltac dec_eq_key_elt :=
-      match goal with
-	H:(eq_key_elt ?a ?b) |- ?c 
-	  => let x:= fresh "eqk" in 
-	    let y := fresh "eqe" in (elim H;clear H;intros x y)
-      end.
-
-    Lemma InList_In_eq_key : forall k e l, InList eq_key (k,e) l -> In k l.
-      unfold eq_key.
-      intros k e l H. 
-      induction H.
-      destruct y.
-      exists e0.
-      eauto.
-      induction IHInList.
-      exists x;eauto.
-    Qed.
-    Hint Resolve InList_In_eq_key.
-
-    (* could also be proved as a corollary of previous lemma *)
-    Lemma InList_In : forall k e l, InList eq_key_elt (k,e) l -> In k l.
-      intros k e l H. exists e;auto.
-    Qed.
-    Hint Resolve InList_In.
-
-   Lemma lt_key_right_r : forall x k e e', lt_key x (k,e) -> lt_key x (k,e').
-      auto.
-    Qed.
-
-    Lemma lt_key_right_l : forall x k e e', lt_key (k,e) x -> lt_key (k,e') x.
-      auto.
-    Qed.
-
-    Hint Resolve lt_key_right_l lt_key_right_r.
-
-    Hint Resolve MX.lt_eq.
-
-    Lemma eq_key_no_lt_key : forall x x', eq_key x x' -> ~lt_key x x'.
-      intros (k,e) (k',e') abs1 abs2.
-      absurd (X.eq k k'); auto.
-    Qed.
-
-    Hint Resolve eq_key_no_lt_key. 
-
-    Lemma eq_key_elt_no_lt_key : forall x x', eq_key_elt x x' -> ~lt_key x x'.
-      intros (k,e) (k',e') abs1.
-      destruct abs1; auto.
-    Qed.
-
-    Hint Resolve eq_key_elt_no_lt_key. 
-
-    Lemma lt_key_trans : forall e e' e'', lt_key e e' -> lt_key e' e'' -> lt_key e e''.
-      eauto.
-    Qed.
-
-    Lemma lt_key_eq_key : forall e e' e'', lt_key e e' -> eq_key e' e'' -> lt_key e e''.
-      intros (k,e) (k',e') (k'',e'').
-      unfold lt_key, eq_key; simpl; intros.
-      eapply MX.lt_eq;eauto.
-    Qed.
-
-    Hint Resolve lt_key_eq_key.
-
-    Lemma eq_key_lt_key : forall e e' e'', lt_key e e'' -> eq_key e e' -> lt_key e' e''.
-      intros (k,e) (k',e') (k'',e'').
-      unfold lt_key, eq_key; simpl; intros.
-      apply MX.eq_lt with k;eauto.
-    Qed.
-
-    Hint Resolve eq_key_lt_key.
-
-    Lemma eq_key_refl : forall e, eq_key e e.
-      auto.
-    Qed.
-
-    Lemma eq_key_elt_refl : forall e, eq_key_elt e e.
-      auto.
-    Qed.
-
-    Lemma eq_key_sym : forall e e', eq_key e e' -> eq_key e' e.
-      auto.
-    Qed.
-
-    Lemma eq_key_elt_sym : forall e e', eq_key_elt e e' -> eq_key_elt e' e.
-      unfold eq_key_elt; intuition.
-    Qed.
-
-    Lemma eq_key_trans : forall e e' e'', eq_key e e' -> eq_key e' e'' -> eq_key e e''.
-      eauto. 
-    Qed.
-
-    Lemma eq_key_elt_trans : forall e e' e'', 
-      eq_key_elt e e' -> eq_key_elt e' e'' -> eq_key_elt e e''.
-      unfold eq_key_elt; intuition eauto; congruence.
-    Qed.
-
-    Hint Resolve eq_key_trans eq_key_elt_trans eq_key_sym eq_key_elt_sym eq_key_refl 
-      eq_key_elt_refl.
-
-    Notation Sort := (sort lt_key).
-    Notation Inf := (lelistA lt_key).
+    Notation Sort := (sort ltk).
+    Notation Inf := (lelistA ltk).
 
     Hint Resolve nil_sort cons_sort.
 
-    Lemma lt_sort_tl : forall e l (sorted:Sort (e::l)), Sort l.
+    Lemma lt_sort_tl : forall e l, Sort (e::l) -> Sort l.
       intros e l sorted.
       inversion sorted.
       inversion H1; auto.
     Qed.
-
      Hint Resolve lt_sort_tl.
 
-    Lemma lt_sort_tl2 : forall e e' l (sorted:Sort (e::e'::l)), Sort (e::l).
+    Lemma lt_sort_tl2 : forall e e' l, Sort (e::e'::l) -> Sort (e::l).
       intros e e' l sorted.
       inversion sorted.
       inversion H1.
@@ -186,91 +207,73 @@ Module Raw (X:OrderedType).
       apply nil_leA.
       apply cons_leA.
       subst.
-      apply lt_key_trans with e';auto.
+      apply ltk_trans with e';auto.
       inversion sorted.
       inversion H4.
       assumption.
     Qed.
-      
     Hint Resolve lt_sort_tl2.
 
     Lemma all_lt_Inf: forall x l, 
-      (forall e, InList eq_key_elt e l -> lt_key x e) -> Inf x l.
-      intros x l H. destruct l;auto.
+      (forall e, InList eqke e l -> ltk x e) -> Inf x l.
+      destruct l;auto.
     Qed.
-
     Hint Resolve all_lt_Inf.
 
-    Lemma sort_in_tl : forall e l e', Sort (e::l) -> InList eq_key e' l -> lt_key e e'.
+    Lemma sort_in_tl : forall e l e', Sort (e::l) -> InList eqk e' l -> ltk e e'.
       intros e l e' sorted Hin.
       induction Hin;eauto.
 
-      apply lt_key_eq_key with y;eauto.
+      apply ltk_eqk with y;eauto.
       inversion sorted.
       subst.
       inversion H3;eauto.
     Qed.
 
-    Lemma sort_in : forall l e e', Sort (e::l) -> InList eq_key e' (e::l) 
-      -> lt_key e e' \/ eq_key e e'.
+    Lemma sort_in : forall l e e', Sort (e::l) -> InList eqk e' (e::l) 
+      -> ltk e e' \/ eqk e e'.
       intros l e e' sorted Hin.
       inversion Hin;eauto.
       left.
       apply sort_in_tl with l;assumption.
     Qed.
 
-    Lemma sort_lt_notin : forall l k e (sorted : Sort l), 
-      Inf (k,e) l ->  ~In k l.
+    Lemma sort_lt_notin : forall l k e, Sort l -> Inf (k,e) l ->  ~In k l.
       intros l k e sorted Hlt.
       inversion Hlt.
       intro abs. inversion abs. inversion H0. 
       intro Hin. subst.
       inversion Hin.
-      assert (lt_key b (k,x) \/ eq_key b (k,x)).
+      assert (ltk b (k,x) \/ eqk b (k,x)).
       eapply sort_in with l0. auto.
       auto.
       decompose [or] H1;clear H1.
-      assert (lt_key (k,x) b).
-      apply lt_key_right_l with e;assumption.
-      absurd (lt_key b (k, x));auto.
+      assert (ltk (k,x) b).
+      apply ltk_right_l with e;assumption.
+      absurd (ltk b (k, x));auto.
       destruct b.
-      unfold lt_key; simpl.
+      unfold ltk; simpl.
       apply MX.lt_not_gt;auto.
 
       destruct b.
-      unfold eq_key in H2; simpl in H2.
-      unfold lt_key in H; simpl in H.
+      unfold eqk in H2; simpl in H2.
+      unfold ltk in H; simpl in H.
       absurd (X.eq k0 k); simpl;eauto.
     Qed.
-
-
-    Lemma sort_lt_notin2 : forall l k e (sorted : Sort l), 
-      Inf (k,e) l -> ~(exists e:elt, InList eq_key (k,e) l).
-      intros l k e sorted Hlt.
-      inversion Hlt.
-      intro abs. inversion abs. inversion H0. 
-      intro Hin. subst.
-      inversion Hin.
-      assert (lt_key b (k,x) \/ eq_key b (k,x)).
-      eapply sort_in with l0. auto.
-      auto.
-      decompose [or] H1;clear H1.
-      assert (lt_key (k,x) b).
-      apply lt_key_right_l with e;assumption.
-      absurd (lt_key b (k, x));auto.
-      destruct b.
-      unfold lt_key; simpl.
-      apply MX.lt_not_gt;auto.
-
-      destruct b.
-      unfold eq_key in H2; simpl in H2.
-      unfold lt_key in H; simpl in H.
-      absurd (X.eq k0 k); simpl;eauto.
-    Qed.
-
     Hint Resolve sort_lt_notin.
 
-    Lemma sorted_unique: forall l, Sort l -> Unique eq_key l.
+(*
+    Lemma sort_lt_notin2 : forall l k e, Sort l -> Inf (k,e) l -> 
+          ~(exists e:elt, InList eqk (k,e) l).
+    Proof.
+      intros.
+      generalize (altern_In k l).
+      generalize (sort_lt_notin H H0).
+      intuition.
+    Qed.
+*)
+
+    Lemma sorted_unique: forall l, Sort l -> Unique eqk l.
       intros l sorted.
       induction sorted;auto.
       apply Unique_cons;auto.
@@ -282,44 +285,30 @@ Module Raw (X:OrderedType).
       eauto.
     Qed.
 
-    Lemma sorted_unique2: forall l, Sort l -> Unique eq_key_elt l.
-      intros l sorted.
-      induction sorted;auto.
-      apply Unique_cons;auto.
-      destruct a;auto.
-      assert (abs:~In k l).
-      eapply sort_lt_notin with e;auto.
-      intro abs2.
-      elim abs.
-      eauto.
+(*
+    Lemma sorted_unique_key_eq: forall l, Unique eqk l -> Unique eqke l.
+      induction 1;auto.
     Qed.
+*)
 
-    Lemma sorted_unique_key_eq: forall l, Unique eq_key l -> Unique eq_key_elt l.
-      intros l unique.
-      induction unique;auto.
-    Qed.
-      
-
-    Lemma Inf_eq : forall x x' l, 
-      eq_key x x' -> Inf x l -> Inf x' l.
+    Lemma Inf_eq : forall x x' l, eqk x x' -> Inf x l -> Inf x' l.
     Proof.  
      intros x x' l H H0.
      inversion H0; eauto.
     Qed.
 
-    Lemma Inf_lt : forall x x' l, lt_key x x' -> Inf x' l -> Inf x l.
+    Lemma Inf_lt : forall x x' l, ltk x x' -> Inf x' l -> Inf x l.
     Proof.
      induction 2; auto.
      constructor.
-     eapply lt_key_trans; eauto.
+     eapply ltk_trans; eauto.
    Qed.     
 
    Hint Resolve Inf_eq Inf_lt.
 
-   Lemma sorted_in_cons_not_eq : forall x l k e (sorted:Sort ((k,e)::l)) (Hin: In x l),
-      ~X.eq x k.
+   Lemma sorted_in_cons_not_eq : forall x l k e, Sort ((k,e)::l) -> In x l -> ~X.eq x k.
       intros x l k e sorted.
-      inversion sorted.
+      inversion_clear sorted.
       intros Hin.
       intro abs.
       absurd (In x l);auto.
@@ -330,26 +319,51 @@ Module Raw (X:OrderedType).
     Lemma In_inv : forall k k' e l, In k ((k',e) :: l) -> X.eq k k' \/ In k l.
       intros k k' e l H.
       inversion H.
-      inversion_clear H0; unfold eq_key_elt in H1; simpl in *; intuition; eauto.
+      inversion_clear H0; unfold eqke in H1; simpl in *; intuition; eauto.
     Qed.      
 
     Lemma In_inv2 : forall x x' l, 
-      InList eq_key x (x' :: l) -> eq_key x x' \/ InList eq_key x l.
+      InList eqk x (x' :: l) -> eqk x x' \/ InList eqk x l.
       intros x x' l inlist.
       inversion inlist;auto.
     Qed.
 
     Lemma In_inv3 : forall x x' l, 
-      InList eq_key_elt x (x' :: l) -> eq_key_elt x x' \/ InList eq_key_elt x l.
+      InList eqke x (x' :: l) -> eqke x x' \/ InList eqke x l.
       intros x x' l inlist.
       inversion inlist;auto.
     Qed.
+
+    Lemma In_inv4 : forall k k' e e' l, 
+      InList eqk (k, e) ((k', e') :: l) -> ~ X.eq k k' -> InList eqk (k, e) l.
+      intros k k' e e' l H H0.
+      elim (@In_inv2 (k,e) (k',e') l);intros;auto.
+      elim H0;auto.
+    Qed.
+
+    Lemma In_inv5 : forall x x' l, 
+      InList eqke x (x' :: l) -> ~ eqk x x' -> InList eqke x l.
+      intros x x' l H H0.
+      induction (@In_inv3 x x' l);auto. 
+      elim H0.
+      unfold eqke in *; unfold eqk; intuition.
+    Qed.
+
+    Lemma InList_eqk : forall x x' l, 
+      InList eqk x l -> eqk x x' -> InList eqk x' l.
+      intros x x' l H H0.
+      induction H;eauto.
+    Qed.
+
+    Hint Resolve In_inv4 In_inv5.
 
    (** end of auxiliary results *)
 
     Definition empty : t elt := [].
 
     (** Specification of [empty] *)
+
+    Definition Empty m := forall (a : key)(e:elt) , ~ MapsTo a e m.
 
     Lemma empty_1 : Empty empty.
       unfold Empty,empty,MapsTo.
@@ -375,7 +389,7 @@ Module Raw (X:OrderedType).
       case m;auto.
       intros p l inlist.
       destruct p.
-      absurd (InList eq_key_elt (k, e) ((k, e) :: l));auto.
+      absurd (InList eqke (k, e) ((k, e) :: l));auto.
     Qed.
 
 
@@ -392,9 +406,9 @@ Module Raw (X:OrderedType).
 	| [] => false
 	| (k',_) :: l =>
           match X.compare k k' with
-            | FSetInterface.Lt _ => false
-            | FSetInterface.Eq _ => true
-            | FSetInterface.Gt _ => mem k l
+            | Lt _ => false
+            | Eq _ => true
+            | Gt _ => mem k l
           end
       end.
     
@@ -430,9 +444,9 @@ Module Raw (X:OrderedType).
 	| [] => None
 	| (k',x)::s' => 
 	  match X.compare k k' with
-	    | (FSetInterface.Lt _) => None
-	    | (FSetInterface.Eq _) => Some x
-	    | (FSetInterface.Gt _) => find k s'
+	    | Lt _ => None
+	    | Eq _ => Some x
+	    | Gt _ => find k s'
 	  end
       end.
 
@@ -452,22 +466,22 @@ Module Raw (X:OrderedType).
       intros; elimtype False.
       inversion_clear H.
       absurd (X.eq k k'); auto.
-      unfold eq_key_elt in H0; simpl in H0; intuition. 
-      assert (H2 := sort_in_tl Hm (InList_eq_key_el_eq_key H0)).
-      unfold lt_key in H2; simpl in H2; intuition. 
+      unfold eqke in H0; simpl in H0; intuition. 
+      assert (H2 := sort_in_tl Hm (InList_eqke_eqk H0)).
+      unfold ltk in H2; simpl in H2; intuition. 
       absurd (X.lt k k'); auto.
     
      intros.
      inversion_clear H.
-     unfold eq_key_elt in H0; simpl in H0; intuition congruence. 
-     assert (H2 := sort_in_tl Hm (InList_eq_key_el_eq_key H0)).
-     unfold lt_key in H2; simpl in H2; intuition. 
+     unfold eqke in H0; simpl in H0; intuition congruence. 
+     assert (H2 := sort_in_tl Hm (InList_eqke_eqk H0)).
+     unfold ltk in H2; simpl in H2; intuition. 
      absurd (X.eq k k'); auto.
 
      intros.
      inversion_clear H0.
      absurd (X.eq k k'); auto.
-     unfold eq_key_elt in H1; simpl in H1; intuition.
+     unfold eqke in H1; simpl in H1; intuition.
      eauto.
     Qed.
 
@@ -477,9 +491,9 @@ Module Raw (X:OrderedType).
 	| [] => (k,x) :: []
 	| (k',y) :: l =>
           match X.compare k k' with
-            | FSetInterface.Lt _ => (k,x)::s
-            | FSetInterface.Eq _ => (k,x)::l
-            | FSetInterface.Gt _ => (k',y) :: add k x l
+            | Lt _ => (k,x)::s
+            | Eq _ => (k,x)::l
+            | Gt _ => (k',y) :: add k x l
           end
       end.
 
@@ -492,29 +506,6 @@ Module Raw (X:OrderedType).
       functional induction add x e m;simpl;auto.
     Qed.
 
-    Lemma aux' : forall k k' e e' l, 
-      InList eq_key (k, e) ((k', e') :: l) -> ~ X.eq k k' -> InList eq_key (k, e) l.
-      intros k k' e e' l H H0.
-      elim (@In_inv2 (k,e) (k',e') l);intros;auto.
-      elim H0;auto.
-    Qed.
-
-    Lemma aux'' : forall x x' l, 
-      InList eq_key_elt x (x' :: l) -> ~ eq_key x x' -> InList eq_key_elt x l.
-      intros x x' l H H0.
-      induction (@In_inv3 x x' l);auto. 
-      elim H0.
-      unfold eq_key_elt in *; unfold eq_key; intuition.
-    Qed.
-
-    Lemma aux''' : forall x x' l, 
-      InList eq_key x l -> eq_key x x' -> InList eq_key x' l.
-      intros x x' l H H0.
-      induction H;eauto.
-    Qed.
-
-    Hint Resolve aux'' aux'.
-
     Lemma add_2 : forall m x y e e', 
       ~ X.eq x y -> MapsTo y e m -> MapsTo y e (add x e' m).
       intros m x  y e e'. 
@@ -522,7 +513,7 @@ Module Raw (X:OrderedType).
       functional induction add x e' m;simpl;auto.
       intros y' e' eqky' mapsto1.
       
-      assert (InList eq_key_elt (y', e') l); intuition; eauto.
+      assert (InList eqke (y', e') l); intuition; eauto.
 
       intros y' e' eqky' mapsto1.
       elim (@In_inv3 (y',e') (k',y) l);auto.
@@ -537,14 +528,14 @@ Module Raw (X:OrderedType).
     Qed.
 
    Lemma add_Inf :
-     forall (m : t elt) (x x':key)(e e':elt), Inf (x',e') m -> lt_key (x',e') (x,e) -> Inf (x',e') (add x e m).
+     forall (m : t elt) (x x':key)(e e':elt), Inf (x',e') m -> ltk (x',e') (x,e) -> Inf (x',e') (add x e m).
    Proof.
      induction m.  
      simpl; intuition.
      intros.
      destruct a as (x'',e'').
      inversion_clear H.
-     unfold lt_key in H0,H1; simpl in H0, H1.
+     unfold ltk in H0,H1; simpl in H0, H1.
      simpl; case (X.compare x x''); intuition.
   Qed.
   Hint Resolve add_Inf.
@@ -565,9 +556,9 @@ Module Raw (X:OrderedType).
 	| [] => []
 	| (k',x) :: l =>
           match X.compare k k' with
-            | FSetInterface.Lt _ => s
-            | FSetInterface.Eq _ => l
-            | FSetInterface.Gt _ => (k',x) :: remove k l
+            | Lt _ => s
+            | Eq _ => l
+            | Gt _ => (k',x) :: remove k l
           end
       end.  
 
@@ -582,7 +573,7 @@ Module Raw (X:OrderedType).
       eapply sort_lt_notin with x.
       eauto.
       apply cons_leA;simpl.
-      unfold lt_key; eapply MX.lt_eq;eauto.
+      unfold ltk; eapply MX.lt_eq;eauto.
       
       eapply sort_lt_notin with x. eauto. 
       inversion Hm.
@@ -592,7 +583,7 @@ Module Raw (X:OrderedType).
       assert (notin:~ In y (remove k l)). apply H;eauto.
       intros (x0,abs).
       inversion_clear abs; eauto. 
-      dec_eq_key_elt; simpl in *; subst.
+      simpl_eqke; simpl in *; subst.
       absurd (X.eq y k');eauto.
       Qed.
       
@@ -607,7 +598,7 @@ Module Raw (X:OrderedType).
       elim (@In_inv3 (y, e) (k', x) l); auto. 
       intro inlist2.
 
-      assert (InList eq_key_elt (y, e) (remove k l));auto.
+      assert (InList eqke (y, e) (remove k l));auto.
       apply H;auto.
       eauto.
     Qed.
@@ -630,11 +621,11 @@ Module Raw (X:OrderedType).
      intros.
      destruct a as (x'',e'').
      inversion_clear H.
-     unfold lt_key in H0; simpl in H0.
+     unfold ltk in H0; simpl in H0.
      simpl; case (X.compare x x''); intuition.
      inversion_clear Hm.
      eapply Inf_lt; eauto.
-     unfold lt_key; auto.
+     unfold ltk; auto.
   Qed.
   Hint Resolve remove_Inf.
 
@@ -656,10 +647,8 @@ Module Raw (X:OrderedType).
       induction inlist;eauto.
 
       apply InList_cons_hd;auto.
-      eapply eq_key_elt_trans with (x, e);auto.
+      eapply eqke_trans with (x, e);auto.
     Qed.
-
-
 
     Fixpoint fold (A:Set) (f:key -> elt -> A -> A) (m:t elt) {struct m} : A -> A :=
       fun acc => 
@@ -674,7 +663,7 @@ Module Raw (X:OrderedType).
 	forall (m: t elt)(Hm:Sort m)(A : Set) (acc : A) (f : key -> elt -> A -> A) ,
 	  exists l : list (key*elt),
             Sort l /\
-            (forall (k:key)(x:elt), MapsTo k x m <-> InList eq_key_elt (k,x) l) 
+            (forall (k:key)(x:elt), MapsTo k x m <-> InList eqke (k,x) l) 
             /\
             fold f m acc = fold_right (fun p => f (fst p) (snd p)) acc l.
         intros m Hm A acc f; generalize Hm; clear Hm.
@@ -696,7 +685,7 @@ Module Raw (X:OrderedType).
 	intros e' hyp.
 	destruct e'.
 	elim (H1 k0 e0);intros .
-	assert (InList eq_key_elt (k0, e0) m').
+	assert (InList eqke (k0, e0) m').
 	apply H4;assumption.
 	eapply sort_in_tl with m';auto.
 
@@ -727,8 +716,8 @@ Module Raw (X:OrderedType).
       Lemma fold_1 :
 	forall (m:t elt)(Hm:Sort m)(A : Set) (acc : A) (f : key -> elt -> A -> A),
 	  exists l : list (key*elt),
-            Unique eq_key l /\
-            (forall (k:key)(x:elt), MapsTo k x m <-> InList eq_key_elt (k,x) l) 
+            Unique eqk l /\
+            (forall (k:key)(x:elt), MapsTo k x m <-> InList eqke (k,x) l) 
             /\
             fold f m acc = fold_right (fun p => f (fst p) (snd p)) acc l.
 	intros m Hm A acc f.
@@ -762,11 +751,13 @@ Module Raw (X:OrderedType).
 
         destruct p as (k,e).
         destruct (H0 k).
-        destruct H2; eauto.
+        destruct H2.
+        exists e; auto.
         inversion H2.
 
         destruct (H0 x).
-        destruct H; eauto.
+        destruct H.
+        exists e; auto.
         inversion H.
 
         subst; clear H_eq_3.
@@ -849,20 +840,19 @@ Module Raw (X:OrderedType).
        inversion_clear Hm; inversion_clear Hm'.
        destruct (H H0 H6 H4).
        inversion_clear H1.
-       dec_eq_key_elt; simpl in *; subst.
+       simpl_eqke; simpl in *; subst.
        inversion_clear H2. 
-       dec_eq_key_elt; simpl in *; subst; auto.
+       simpl_eqke; simpl in *; subst; auto.
        elim (sort_lt_notin H6 H7).
        exists e'0; apply MapsTo_1 with k; eauto.
        inversion_clear H2. 
-       dec_eq_key_elt; simpl in *; subst; auto.
+       simpl_eqke; simpl in *; subst; auto.
        elim (sort_lt_notin H0 H5).
        exists e1; apply MapsTo_1 with k; eauto.
        apply H9 with k; eauto.
       Qed. 
-      
 
-      Variable elt' elt'':Set.
+      Variable elt':Set.
       
       Fixpoint map (f:elt -> elt') (m:t elt) {struct m} : t elt' :=
 	match m with
@@ -876,6 +866,150 @@ Module Raw (X:OrderedType).
 	  | (k,e)::m' => (k,f k e) :: mapi f m'
 	end.
 
+      End Elt.
+      Section Elt2. 
+      (* For previous definitions to work with different [elt], especially [MapsTo]... *)
+      
+      Variable elt elt' : Set.
+
+    (** Specification of [map] *)
+
+      Lemma map_1 : forall (m:t elt)(x:key)(e:elt)(f:elt->elt'), 
+        MapsTo x e m -> MapsTo x (f e) (map f m).
+      Proof.
+	intros m x e f.
+	(* functional induction map elt elt' f m.  *) (* Marche pas ??? *)
+        induction m.
+        inversion 1.
+        
+        destruct a as (x',e').
+        simpl. 
+        inversion_clear 1.
+        constructor 1.
+        unfold eqke in *; simpl in *; intuition congruence.
+        constructor 2.
+        unfold MapsTo in *; auto.
+      Qed.
+
+      Lemma map_2 : forall (m:t elt)(x:key)(f:elt->elt'), 
+        In x (map f m) -> In x m.
+      Proof.
+	intros m x f. 
+        (* functional induction map elt elt' f m. *) (* Marche pas ??? *)
+        induction m; simpl.
+        intros (e,abs).
+        inversion abs.
+        
+        destruct a as (x',e).
+	intros hyp.
+	inversion hyp. clear hyp.
+	inversion H; subst; rename x0 into e'.
+        exists e; constructor.
+        unfold eqke in *; simpl in *; intuition.
+        destruct IHm as (e'',hyp).
+        exists e'; auto.
+        exists e''.
+        constructor 2; auto.
+      Qed.
+
+      Lemma map_lelistA : 
+         forall (m: t elt)(x:key)(e:elt)(e':elt')(f:elt->elt'),
+         lelistA (@ltk elt) (x,e) m -> 
+         lelistA (@ltk elt') (x,e') (map f m).
+      Proof. 
+        induction m; simpl; auto.
+        intros.
+        destruct a as (x0,e0).
+        inversion_clear H; auto.
+      Qed.
+
+      Hint Resolve map_lelistA.
+
+      Lemma map_sorted : 
+         forall (m: t elt)(Hm : sort (@ltk elt) m)(f:elt -> elt'), 
+         sort (@ltk elt') (map f m).
+      Proof.   
+      induction m; simpl; auto.
+      intros.
+      destruct a as (x',e').
+      inversion_clear Hm; eauto.
+      Qed.      
+      
+ 
+    (** Specification of [mapi] *)
+
+      Lemma mapi_1 : forall (m:t elt)(x:key)(e:elt)
+        (f:key->elt->elt'), MapsTo x e m -> 
+        exists y, X.eq y x /\ MapsTo x (f y e) (mapi f m).
+      Proof.
+	intros m x e f.
+	(* functional induction mapi elt elt' f m. *) (* Marche pas ??? *)
+        induction m.
+        inversion 1.
+        
+        destruct a as (x',e').
+        simpl. 
+        inversion_clear 1.
+        exists x'.
+        destruct H0; simpl in *.
+        split; auto.
+        constructor 1.
+        unfold eqke in *; simpl in *; intuition congruence.
+        destruct IHm as (y, hyp); auto.
+        exists y; intuition.
+        constructor 2.
+        unfold MapsTo in *; auto.
+      Qed.  
+
+
+      Lemma mapi_2 : forall (m:t elt)(x:key)
+        (f:key->elt->elt'), In x (mapi f m) -> In x m.
+      Proof.
+	intros m x f. 
+        (* functional induction mapi elt elt' f m. *) (* Marche pas ??? *)
+        induction m; simpl.
+        intros (e,abs).
+        inversion abs.
+        
+        destruct a as (x',e).
+	intros hyp.
+	inversion hyp. clear hyp.
+	inversion H; subst; rename x0 into e'.
+        exists e; constructor.
+        unfold eqke in *; simpl in *; intuition.
+        destruct IHm as (e'',hyp).
+        exists e'; auto.
+        exists e''.
+        constructor 2; auto.
+      Qed.
+
+      Lemma mapi_lelistA : 
+         forall (m: t elt)(x:key)(e:elt)(f:key->elt->elt'),
+         lelistA (@ltk elt) (x,e) m -> 
+         lelistA (@ltk elt') (x,f x e) (mapi f m).
+      Proof. 
+        induction m; simpl; auto.
+        intros.
+        destruct a as (x',e').
+        inversion_clear H; auto.
+      Qed.
+
+      Hint Resolve mapi_lelistA.
+
+      Lemma mapi_sorted : 
+         forall (m: t elt)(Hm : sort (@ltk elt) m)(f: key ->elt -> elt'), 
+         sort (@ltk elt') (mapi f m).
+      Proof.
+      induction m; simpl; auto.
+      intros.
+      destruct a as (x',e').
+      inversion_clear Hm; auto.
+      Qed.
+
+    End Elt2. 
+    Section Elt3.
+
+      Variable elt elt' elt'' : Set.
       Variable f : option elt -> option elt' -> option elt''.
 
       Definition option_cons (A:Set)(k:key)(o:option A)(l:list (key*A)) := 
@@ -889,7 +1023,7 @@ Module Raw (X:OrderedType).
           | [] => [] 
           | (k,e)::l => option_cons k (f (Some e) None) (map2_l l)
         end. 
- 
+
       Fixpoint map2_r (m' : t elt') : t elt'' := 
         match m' with 
           | [] => [] 
@@ -898,241 +1032,331 @@ Module Raw (X:OrderedType).
 
       Fixpoint map2 (m : t elt) : t elt' -> t elt'' :=
         match m with
-          | [] => map2_r
+          | [] => map2_r 
           | (k,e) :: l =>
             fix map2_aux (m' : t elt') : t elt'' :=
               match m' with
                 | [] => map2_l m
                 | (k',e') :: l' =>
                   match X.compare k k' with
-                    | FSetInterface.Lt _ => option_cons k (f (Some e) None) (map2 l m')
-                    | FSetInterface.Eq _ => option_cons k (f (Some e) (Some e')) (map2 l l')
-                    | FSetInterface.Gt _ => option_cons k' (f None (Some e')) (map2_aux l')
+                    | Lt _ => option_cons k (f (Some e) None) (map2 l m')
+                    | Eq _ => option_cons k (f (Some e) (Some e')) (map2 l l')
+                    | Gt _ => option_cons k' (f None (Some e')) (map2_aux l')
                   end
               end
         end.      
 
+     Fixpoint combine (m : t elt) : t elt' -> t (option elt * option elt') :=
+        match m with
+          | [] => map (fun e' => (None,Some e'))
+          | (k,e) :: l =>
+            fix combine_aux (m' : t elt') : list (key * (option elt * option elt')) :=
+              match m' with
+                | [] => map (fun e => (Some e,None)) m
+                | (k',e') :: l' =>
+                  match X.compare k k' with
+                    | Lt _ => (k,(Some e, None))::combine l m'
+                    | Eq _ => (k,(Some e, Some e'))::combine l l'
+                    | Gt _ => (k',(None,Some e'))::combine_aux l'
+                  end
+              end
+        end. 
 
-  End Elt.
+    Definition map2_alt m m' := 
+      let m0 : t (option elt * option elt') := combine m m' in 
+      let m1 : t (option elt'') := map (fun p => f (fst p) (snd p)) m0 in 
+      fold (option_cons (A:=elt'')) m1 nil.
 
-    (** Specification of [map] *)
+    Lemma map2_alt_equiv : 
+      forall m m', map2_alt m m' = map2 m m'.
+    Proof.
+    unfold map2_alt.
+    induction m.
+    simpl; auto; intros.
+    (* map2_r *)
+    induction m'; try destruct a; simpl; auto.
+    rewrite IHm'; auto.
+    (* fin map2_r *)
+    induction m'; destruct a.
+    simpl; f_equal.
+    (* map2_l *)
+    clear IHm.
+    induction m; try destruct a; simpl; auto.
+    rewrite IHm; auto.
+    (* fin map2_l *)
+    destruct a0.
+    simpl.
+    destruct (X.compare t0 t1); simpl; f_equal.
+    apply IHm.
+    apply IHm.
+    apply IHm'.
+    Qed.
 
-      Lemma map_1 : forall (elt elt':Set)(m:t elt)(x:key)(e:elt)(f:elt->elt'), 
-        MapsTo x e m -> MapsTo x (f e) (map f m).
-      Proof.
-	intros elt elt' m x e f.
-	(* functional induction map elt elt' f m.  *) (* Marche pas ??? *)
-        induction m.
-        inversion 1.
-        
-        destruct a as (x',e').
-        simpl. 
-        inversion_clear 1.
-        constructor 1.
-        unfold eq_key_elt in *; simpl in *; intuition congruence.
-        constructor 2.
-        unfold MapsTo in *; auto.
-      Qed.
+   Lemma combine_lelistA : 
+      forall (m: t elt)(m': t elt')(x:key)(e:elt)(e':elt')(e'':option elt * option elt'), 
+        lelistA (@ltk elt) (x,e) m -> 
+        lelistA (@ltk elt') (x,e') m' -> 
+        lelistA (@ltk (option elt * option elt')) (x,e'') (combine m m').
+    Proof.
+    induction m. 
+    intros.
+    simpl.
+    eapply map_lelistA; eauto.
+    induction m'. 
+    intros.
+    destruct a.
+    replace (combine ((t0, e0) :: m) []) with 
+                 (map (fun e => (Some e,None (A:=elt'))) ((t0,e0)::m)); auto.
+    eapply map_lelistA; eauto.
+    intros.
+    simpl.
+    destruct a as (k,e0); destruct a0 as (k',e0').
+    destruct (X.compare k k').
+    inversion_clear H; auto.
+    inversion_clear H; auto.
+    inversion_clear H0; auto.
+    Qed.
+    Hint Resolve combine_lelistA.
 
-      Lemma map_2 : forall (elt elt':Set)(m:t elt)(x:key)(f:elt->elt'), 
-        In x (map f m) -> In x m.
-      Proof.
-	intros elt elt' m x f. 
-        (* functional induction map elt elt' f m. *) (* Marche pas ??? *)
-        induction m; simpl.
-        intros (e,abs).
-        inversion abs.
-        
-        destruct a as (x',e).
-	intros hyp.
-	inversion hyp. clear hyp.
-	inversion H; subst; rename x0 into e'.
-        exists e; constructor.
-        unfold eq_key_elt in *; simpl in *; intuition.
-        destruct IHm as (e'',hyp).
-        exists e'; auto.
-        exists e''.
-        constructor 2; auto.
-      Qed.
-
-      Lemma map_lelistA : 
-         forall (elt elt':Set)(m: t elt)(x:key)(e:elt)(f:elt->elt'),
-         lelistA (@lt_key elt) (x,e) m -> 
-         lelistA (@lt_key elt') (x,f e) (map f m).
-      Proof. 
-        induction m; simpl; auto.
-        intros.
-        destruct a as (x',e').
-        inversion_clear H; auto.
-      Qed.
-
-      Hint Resolve map_lelistA.
-
-      Lemma map_sorted : 
-         forall (elt elt':Set)(m: t elt)(Hm : sort (@lt_key elt) m)(f:elt -> elt'), 
-         sort (@lt_key elt') (map f m).
-      Proof.   
-      induction m; simpl; auto.
-      intros.
-      destruct a as (x',e').
-      inversion_clear Hm; auto.
-      Qed.      
-      
- 
-    (** Specification of [mapi] *)
-
-      Lemma mapi_1 : forall (elt elt':Set)(m:t elt)(x:key)(e:elt)
-        (f:key->elt->elt'), MapsTo x e m -> 
-        exists y, X.eq y x /\ MapsTo x (f y e) (mapi f m).
-      Proof.
-	intros elt elt' m x e f.
-	(* functional induction mapi elt elt' f m. *) (* Marche pas ??? *)
-        induction m.
-        inversion 1.
-        
-        destruct a as (x',e').
-        simpl. 
-        inversion_clear 1.
-        exists x'.
-        destruct H0; simpl in *.
-        split; auto.
-        constructor 1.
-        unfold eq_key_elt in *; simpl in *; intuition congruence.
-        destruct IHm as (y, hyp); auto.
-        exists y; intuition.
-        constructor 2.
-        unfold MapsTo in *; auto.
-      Qed.  
-
-
-      Lemma mapi_2 : forall (elt elt':Set)(m:t elt)(x:key)
-        (f:key->elt->elt'), In x (mapi f m) -> In x m.
-      Proof.
-	intros elt elt' m x f. 
-        (* functional induction mapi elt elt' f m. *) (* Marche pas ??? *)
-        induction m; simpl.
-        intros (e,abs).
-        inversion abs.
-        
-        destruct a as (x',e).
-	intros hyp.
-	inversion hyp. clear hyp.
-	inversion H; subst; rename x0 into e'.
-        exists e; constructor.
-        unfold eq_key_elt in *; simpl in *; intuition.
-        destruct IHm as (e'',hyp).
-        exists e'; auto.
-        exists e''.
-        constructor 2; auto.
-      Qed.
-
-      Lemma mapi_lelistA : 
-         forall (elt elt':Set)(m: t elt)(x:key)(e:elt)(f:key->elt->elt'),
-         lelistA (@lt_key elt) (x,e) m -> 
-         lelistA (@lt_key elt') (x,f x e) (mapi f m).
-      Proof. 
-        induction m; simpl; auto.
-        intros.
-        destruct a as (x',e').
-        inversion_clear H; auto.
-      Qed.
-
-      Hint Resolve mapi_lelistA.
-
-      Lemma mapi_sorted : 
-         forall (elt elt':Set)(m: t elt)(Hm : sort (@lt_key elt) m)(f: key ->elt -> elt'), 
-         sort (@lt_key elt') (mapi f m).
-      Proof.   
-      induction m; simpl; auto.
-      intros.
-      destruct a as (x',e').
-      inversion_clear Hm; auto.
-      Qed.      
-
-     Lemma map2_r_1 : forall (elt elt' elt'':Set)
-        (m': t elt')(Hm' : sort (@lt_key elt') m')
-	(x:key)(f:option elt->option elt'->option elt''), 
-        (In x m' -> find x (map2_r f m') = f None (find x m'))
-        /\
-        (In x (map2_r f m') -> In x m'). 
+    Lemma combine_sorted : 
+      forall (m: t elt)(Hm : sort (@ltk elt) m)(m': t elt')(Hm' : sort (@ltk elt') m'), 
+      sort (@ltk (option elt * option elt')) (combine m m').
+    Proof.
+    induction m. 
+    intros; clear Hm.
+    simpl.
+    apply map_sorted; auto.
+    induction m'. 
+    intros; clear Hm'.
+    destruct a.
+    replace (combine ((t0, e) :: m) []) with 
+                 (map (fun e => (Some e,None (A:=elt'))) ((t0,e)::m)); auto.
+    apply map_sorted; auto.
+    intros.
+    simpl.
+    destruct a as (k,e); destruct a0 as (k',e').
+    destruct (X.compare k k').
+    inversion_clear Hm.
+    constructor; auto.
+    eapply combine_lelistA with (e':=e'); eauto.
+    inversion_clear Hm; inversion_clear Hm'.
+    constructor; eauto.
+    eapply combine_lelistA with (e':=e'); eauto.
+    eapply Inf_eq; eauto; red; eauto.
+    inversion_clear Hm; inversion_clear Hm'.
+    constructor; auto.
+    change (lelistA (ltk (elt:=option elt * option elt')) (k', (None, Some e'))
+                     (combine ((k,e)::m) m')).
+    eapply combine_lelistA with (e:=e); eauto.
+    Qed.
+    
+    Lemma map2_sorted : 
+      forall (m: t elt)(Hm : sort (@ltk elt) m)(m': t elt')(Hm' : sort (@ltk elt') m'), 
+      sort (@ltk elt'') (map2 m m').
      Proof.
-     induction m'.
      intros.
-     split; simpl; destruct 1; inversion H.
-     destruct a as (k',e').
-     split; simpl; intros.
-     unfold option_cons.
-     destruct H as (e,H).
-     inversion_clear H. 
-     destruct H0; simpl in *; subst. 
-     destruct (X.compare x k'); try solve [absurd (X.eq x k'); eauto]. 
-     destruct (f None (Some e')); simpl.
-     destruct (X.compare x k'); try solve [absurd (X.eq x k'); eauto]; auto. 
-     inversion_clear Hm'.
-     destruct (IHm' H0 k' f) as (_,H2).
-     case_eq (find x (map2_r f m')); auto; intros.
-     absurd (In k' m').
-     eapply sort_lt_notin; eauto.
-     apply H2.
-     exists e0.
-     apply MapsTo_1 with x; auto.
-     apply find_2; auto.
-     inversion_clear Hm'.
-     destruct (IHm' H x f) as (H2,H3).
-     assert (X.lt k' x).
-       admit. (* TODO *)
-     destruct (X.compare x k'); try solve [absurd (X.lt k' x); eauto].
-     destruct (f None (Some e')); simpl.
-     destruct (X.compare x k'); try solve [absurd (X.lt k' x); eauto].
-     apply H2; exists e; auto.
-     apply H2; exists e; auto.
-     unfold option_cons in H.
-     destruct (f None (Some e')).
-     destruct H.
+     rewrite <- map2_alt_equiv.
+     unfold map2_alt.
+     assert (H0:=combine_sorted Hm Hm').
+     set (l0:=combine m m') in *; clearbody l0.
+     set (f':= fun p : option elt * option elt' => f (fst p) (snd p)).
+     assert (H1:=map_sorted (elt' := option elt'') H0 f').
+     set (l1:=map f' l0) in *; clearbody l1. 
+     clear f' f H0 l0 Hm Hm' m m'.
+     induction l1.
+     simpl; auto.
+     inversion_clear H1.
+     destruct a; destruct o; auto.
+     simpl.
+     constructor; auto.
+     clear IHl1.
+     induction l1.
+     simpl; auto.
+     destruct a; destruct o; simpl; auto.
+     inversion_clear H0; auto.
+     inversion_clear H0.
+     red in H1; simpl in H1.
      inversion_clear H.
-     destruct H0; simpl in *; subst.
-     exists e'; eauto.
-     constructor; split; simpl; auto.
-     inversion_clear Hm'.
-     destruct (IHm' H x f) as (H2,H3).
-     destruct H3 as (e'',H4).
-     exists x0; auto.
-     exists e''.
-     constructor 2; auto.
-     inversion_clear Hm'.
-     destruct (IHm' H0 x f) as (H2,H3).
-     destruct H3 as (e'',H4); auto.
-     exists e''.
-     constructor 2; auto.
+     apply IHl1; auto.
+     eapply Inf_lt; eauto.
+     red; auto.
      Qed.
+     
+     Definition at_least_one (o:option elt)(o':option elt') := 
+         match o, o' with 
+           | None, None => None 
+           | _, _  => Some (o,o')
+         end.
+
+    Lemma combine_1 : 
+      forall (m: t elt)(Hm : sort (@ltk elt) m)(m': t elt')(Hm' : sort (@ltk elt') m') 
+      (x:key), 
+      find x (combine m m') = at_least_one (find x m) (find x m'). 
+    Proof.
+    induction m.
+    intros.
+    simpl.
+    induction m'.
+    intros; simpl; auto.
+    simpl; destruct a.
+    simpl; destruct (X.compare x t0); simpl; auto.
+    inversion_clear Hm'; auto.
+    induction m'.
+    (* m' = [] *)
+    intros; destruct a; simpl.
+    destruct (X.compare x t0); simpl; auto.
+    inversion_clear Hm; clear H0 l Hm' IHm t0.
+    induction m; simpl; auto.
+    inversion_clear H.
+    destruct a.
+    simpl; destruct (X.compare x t0); simpl; auto.
+    (* m' <> [] *)
+    intros.
+    destruct a as (k,e); destruct a0 as (k',e'); simpl.
+    inversion Hm; inversion Hm'; subst.
+    destruct (X.compare k k'); simpl;
+      destruct (X.compare x k); 
+        MX.compare || destruct (X.compare x k'); simpl; auto.
+    absurd_hyp l; eauto.
+    rewrite IHm; auto; simpl; MX.compare; auto.
+    rewrite IHm; auto; simpl; MX.compare; auto.
+    rewrite IHm; auto; simpl; MX.compare; auto.
+    absurd_hyp e0; eauto.
+    absurd_hyp e0; eauto.
+    change ((find x (combine ((k, e) :: m) m')) = at_least_one None (find x m')).
+    rewrite IHm'; auto. 
+    simpl find; MX.compare; auto.
+    absurd_hyp e0; eauto.
+    absurd_hyp l; eauto.
+    change ((find x (combine ((k, e) :: m) m')) = Some (Some e, find x m')).
+    rewrite IHm'; auto. 
+    simpl find; MX.compare; auto.
+    change ((find x (combine ((k, e) :: m) m')) = at_least_one (find x m) (find x m')).
+    rewrite IHm'; auto. 
+    simpl find; MX.compare; auto.
+    Qed.
+
+    Definition at_least_one_then_f (o:option elt)(o':option elt') := 
+         match o, o' with 
+           | None, None => None 
+           | _, _  => f o o'
+         end.
+
+    Lemma map2_0 : 
+      forall (m: t elt)(Hm : sort (@ltk elt) m)(m': t elt')(Hm' : sort (@ltk elt') m') 
+      (x:key), 
+      find x (map2 m m') = at_least_one_then_f (find x m) (find x m'). 
+    Proof.
+    intros.
+    rewrite <- map2_alt_equiv.
+    unfold map2_alt.
+    assert (H:=combine_1 Hm Hm' x).
+    assert (H2:=combine_sorted Hm Hm').
+    set (f':= fun p : option elt * option elt' => f (fst p) (snd p)).
+    set (m0 := combine m m') in *; clearbody m0.
+    set (o:=find x m) in *; clearbody o. 
+    set (o':=find x m') in *; clearbody o'.
+    clear Hm Hm' m m'.
+    generalize H; clear H.
+    match goal with |- ?g => 
+       assert (g /\ (find x m0 = None -> 
+                           find x (fold (option_cons (A:=elt'')) (map f' m0) []) = None)); 
+       [ | intuition ] end.
+    induction m0; simpl in *; intuition.
+    destruct o; destruct o'; simpl in *; try discriminate; auto.
+    destruct a as (k,(oo,oo')); simpl in *.
+    inversion_clear H2.
+    destruct (X.compare x k); simpl in *.
+    (* x < k *)
+    destruct (f' (oo,oo')); simpl.
+    MX.compare.
+    destruct o; destruct o'; simpl in *; try discriminate; auto.
+    destruct (IHm0 H0) as (H2,_); apply H2; auto.
+    rewrite <- H.
+    case_eq (find x m0); intros; auto.
+    assert (ltk (elt:=option elt * option elt') (x,(oo,oo')) (k,(oo,oo'))).
+     red; auto.
+    destruct (sort_lt_notin H0 (Inf_lt H4 H1)).
+    exists p; apply find_2; eauto.
+    (* x = k *)
+    assert (at_least_one_then_f o o' = f oo oo').
+      destruct o; destruct o'; simpl in *; inversion_clear H; auto.
+    rewrite H2.
+    unfold f'; simpl.
+    destruct (f oo oo'); simpl.
+    MX.compare; auto.
+    destruct (IHm0 H0) as (_,H4); apply H4; auto.
+    case_eq (find x m0); intros; auto.
+    assert (eqk (elt:=option elt * option elt') (k,(oo,oo')) (x,(oo,oo'))).
+     red; auto.
+    destruct (sort_lt_notin H0 (Inf_eq H5 H1)).
+    exists p; apply find_2; eauto.
+    (* k < x *)
+    unfold f'; simpl.
+    destruct (f oo oo'); simpl.
+    MX.compare; auto.
+    destruct (IHm0 H0) as (H3,_); apply H3; auto.
+    destruct (IHm0 H0) as (H3,_); apply H3; auto.
+
+    (* None -> None *)
+    destruct a as (k,(oo,oo')).
+    simpl.
+    inversion_clear H2.
+    destruct (X.compare x k).
+    (* x < k *)
+    unfold f'; simpl.
+    destruct (f oo oo'); simpl.
+    MX.compare; auto.
+    destruct (IHm0 H0) as (_,H4); apply H4; auto.
+    case_eq (find x m0); intros; auto.
+    assert (ltk (elt:=option elt * option elt') (x,(oo,oo')) (k,(oo,oo'))).
+     red; auto.
+    destruct (sort_lt_notin H0 (Inf_lt H3 H1)).
+    exists p; apply find_2; eauto.
+    (* x = k *)
+    discriminate.
+    (* k < x *)
+    unfold f'; simpl.
+    destruct (f oo oo'); simpl.
+    MX.compare; auto.
+    destruct (IHm0 H0) as (_,H4); apply H4; auto.
+    destruct (IHm0 H0) as (_,H4); apply H4; auto.
+    Qed.
 
      (** Specification of [map2] *)
-     Lemma map2_1 : forall (elt elt' elt'':Set)(m: t elt)(Hm : sort (@lt_key elt) m)
-        (m': t elt')(Hm' : sort (@lt_key elt') m')
-	(x:key)(f:option elt->option elt'->option elt''), 
+     Lemma map2_1 : forall (m: t elt)(Hm : sort (@ltk elt) m)
+        (m': t elt')(Hm' : sort (@ltk elt') m')(x:key),
 	In x m \/ In x m' -> 
-        find x (map2 f m m') = f (find x m) (find x m'). 
+        find x (map2 m m') = f (find x m) (find x m'). 
      Proof.
-     induction m.
-     simpl; intros.
-     clear Hm.
-     destruct H.
-     destruct H.
-     inversion H.
-     Admitted.
+     intros.
+     rewrite map2_0; auto.
+     destruct H as [(e,H)|(e,H)].
+     rewrite (find_1 Hm H).
+     destruct (find x m'); simpl; auto.
+     rewrite (find_1 Hm' H).
+     destruct (find x m); simpl; auto.
+     Qed.
+     
+     Lemma map2_2 : forall (m: t elt)(Hm : sort (@ltk elt) m)
+        (m': t elt')(Hm' : sort (@ltk elt') m')(x:key), 
+        In x (map2 m m') -> In x m \/ In x m'. 
+     Proof.
+     intros.
+     destruct H as (e,H).
+     generalize (map2_0 Hm Hm' x).
+     rewrite (find_1 (map2_sorted Hm Hm') H).
+     generalize (@find_2 _ m x).
+     generalize (@find_2 _ m' x).
+     destruct (find x m); 
+       destruct (find x m'); simpl; intros.
+     left; exists e0; auto. 
+     left; exists e0; auto.
+     right; exists e0; auto.
+     discriminate.
+     Qed.
 
-     Lemma map2_2 : forall (elt elt' elt'':Set)(m: t elt)(Hm : sort (@lt_key elt) m)
-        (m': t elt')(Hm' : sort (@lt_key elt') m')
-	(x:key)(f:option elt->option elt'->option elt''), 
-        In x (map2 f m m') -> In x m \/ In x m'.
-     Admitted.
-
-     Lemma map2_sorted : forall (elt elt' elt'':Set)(m: t elt)(Hm : sort (@lt_key elt) m)
-        (m': t elt')(Hm' : sort (@lt_key elt') m')
-        (f:option elt->option elt'->option elt''), 
-        sort (@lt_key elt'') (map2 f m m').
-     Admitted.
-
+   End Elt3.
 
 End Raw.
 
@@ -1143,7 +1367,7 @@ Module Make (X: OrderedType) <: S with Definition key := X.t with Definition keq
   Definition key := X.t. 
   Definition keq := X.eq.
 
-  Record slist (elt:Set) : Set :=  {this :> Raw.t elt; sorted : sort (@Raw.lt_key elt) this}.
+  Record slist (elt:Set) : Set :=  {this :> Raw.t elt; sorted : sort (@Raw.ltk elt) this}.
   Definition t (elt:Set) := slist elt. 
 
  Section Elt. 
@@ -1160,7 +1384,7 @@ Module Make (X: OrderedType) <: S with Definition key := X.t with Definition keq
  Definition map f m : t elt' := Build_slist (Raw.map_sorted m.(sorted) f).
  Definition mapi f m : t elt' := Build_slist (Raw.mapi_sorted m.(sorted) f).
  Definition map2 f m (m':t elt') : t elt'' := 
-     Build_slist (Raw.map2_sorted m.(sorted) m'.(sorted) f).
+     Build_slist (Raw.map2_sorted f m.(sorted) m'.(sorted)).
  Definition fold A f m i := @Raw.fold elt A f m.(this) i.
  Definition equal cmp m m' := @Raw.equal elt cmp m.(this) m'.(this).
 
@@ -1203,10 +1427,10 @@ Module Make (X: OrderedType) <: S with Definition key := X.t with Definition keq
  Definition mapi_1 m := @Raw.mapi_1 elt elt' m.(this).
  Definition mapi_2 m := @Raw.mapi_2 elt elt' m.(this).
 
- Definition map2_1 m (m':t elt') := 
-    @Raw.map2_1 elt elt' elt'' m.(this) m.(sorted) m'.(this) m'.(sorted).
- Definition map2_2 m (m':t elt') := 
-    @Raw.map2_2 elt elt' elt'' m.(this) m.(sorted) m'.(this) m'.(sorted).
+ Definition map2_1 m (m':t elt') x f := 
+    @Raw.map2_1 elt elt' elt'' f m.(this) m.(sorted) m'.(this) m'.(sorted) x.
+ Definition map2_2 m (m':t elt') x f := 
+    @Raw.map2_2 elt elt' elt'' f m.(this) m.(sorted) m'.(this) m'.(sorted) x.
 
  Definition equal_1 m m' := @Raw.equal_1 elt m.(this) m.(sorted) m'.(this) m'.(sorted).
  Definition equal_2 m m' := @Raw.equal_2 elt m.(this) m.(sorted) m'.(this) m'.(sorted).
@@ -1272,14 +1496,14 @@ Module Make_ord (X: OrderedType)(Data : OrderedType) <:
   unfold equal; simpl. 
   destruct (X.compare x x'); simpl; intuition.
   unfold cmp at 1. 
-  destruct (Data.compare e e'); simpl; intuition. 
-  absurd (Data.lt e e'); eauto.
+  MD.compare; clear H; simpl.
   inversion_clear Hl.
   inversion_clear Hl'.
   destruct (IHl H (Build_slist H3)).
   unfold equal, eq in H5; simpl in H5; auto.
-  absurd (Data.lt e' e); eauto.
-  unfold cmp in H; destruct (Data.compare e e'); simpl in H; auto; discriminate.
+  destruct (andb_prop _ _ H); clear H.
+  generalize H0; unfold cmp.
+  MD.compare; auto; intro; discriminate.
   destruct (andb_prop _ _ H); clear H.
   inversion_clear Hl.
   inversion_clear Hl'.
@@ -1319,10 +1543,9 @@ Module Make_ord (X: OrderedType)(Data : OrderedType) <:
      intros (m,Hm); induction m; 
      intros (m', Hm'); destruct m'; unfold eq; simpl;
      try destruct a as (x,e); try destruct p as (x',e'); auto.
-     destruct (X.compare x x'); destruct (X.compare x' x); intuition; 
-      try solve [absurd (X.eq x x'); eauto]. 
+     destruct (X.compare x x'); MapS.Raw.MX.compare; intuition.
      inversion_clear Hm; inversion_clear Hm'.
-     apply (IHm H (Build_slist H3)); auto.
+     apply (IHm H0 (Build_slist H4)); auto.
   Qed.
 
   Lemma eq_trans : forall m1 m2 m3 : t, eq m1 m2 -> eq m2 m3 -> eq m1 m3.
@@ -1334,14 +1557,11 @@ Module Make_ord (X: OrderedType)(Data : OrderedType) <:
      try destruct p0 as (x'',e''); try contradiction; auto.
      destruct (X.compare x x'); 
        destruct (X.compare x' x''); 
-         destruct (X.compare x x''); intros; auto; 
-            try solve [ contradiction | 
-                            absurd (X.lt x x''); eauto | 
-                            absurd (X.lt x' x''); eauto | 
-                            absurd (X.lt x'' x'); eauto ].
-    split; intuition eauto.
+         MapS.Raw.MX.compare.
+     intuition.
+     eauto.
      inversion_clear Hm1; inversion_clear Hm2; inversion_clear Hm3.
-     apply (IHm1 H0 (Build_slist H5) (Build_slist H7)); intuition.
+     apply (IHm1 H1 (Build_slist H6) (Build_slist H8)); intuition.
    Qed.
 
   Lemma lt_trans : forall m1 m2 m3 : t, lt m1 m2 -> lt m2 m3 -> lt m1 m3.
@@ -1354,16 +1574,13 @@ Module Make_ord (X: OrderedType)(Data : OrderedType) <:
      try destruct p0 as (x'',e''); try contradiction; auto.
      destruct (X.compare x x'); 
        destruct (X.compare x' x''); 
-         destruct (X.compare x x''); intros; auto; 
-            try solve [ contradiction | 
-                            absurd (X.lt x x''); eauto | 
-                            absurd (X.lt x' x''); eauto | 
-                            absurd (X.lt x'' x'); eauto ].
+         MapS.Raw.MX.compare; auto.
+    absurd (X.lt x' x''); eauto.
     intuition; try solve [left; eauto].
     right. 
     split; eauto.
      inversion_clear Hm1; inversion_clear Hm2; inversion_clear Hm3.
-     apply (IHm1 H1 (Build_slist H5) (Build_slist H7)); intuition.
+     apply (IHm1 H2 (Build_slist H6) (Build_slist H8)); intuition.
    Qed.
 
   Lemma lt_not_eq : forall m1 m2 : t, lt m1 m2 -> ~ eq m1 m2.
@@ -1391,21 +1608,16 @@ Module Make_ord (X: OrderedType)(Data : OrderedType) <:
     destruct (Data.compare e e').
     apply Lt; unfold lt; simpl;
      destruct (X.compare x x'); auto; absurd (X.eq x x'); eauto.
-    assert (Hm11 : sort (Raw.lt_key (elt:=Data.t)) m1).
+    assert (Hm11 : sort (Raw.ltk (elt:=Data.t)) m1).
      inversion_clear Hm1; auto.
-    assert (Hm22 : sort (Raw.lt_key (elt:=Data.t)) m2).
+    assert (Hm22 : sort (Raw.ltk (elt:=Data.t)) m2).
      inversion_clear Hm2; auto.
     destruct (IHm1 Hm11 (Build_slist Hm22)).
-    apply Lt; unfold lt; simpl; 
-      destruct (X.compare x x'); try (right; auto); absurd (X.eq x x'); eauto.
-    apply Eq; unfold eq; simpl; 
-       destruct (X.compare x x'); auto; absurd (X.eq x x'); eauto.
-    apply Gt; unfold lt; simpl;
-     destruct (X.compare x' x); auto; absurd (X.eq x x'); eauto.
-    apply Gt; unfold lt; simpl;
-     destruct (X.compare x' x); auto; absurd (X.eq x x'); eauto.
-    apply Gt; unfold lt; simpl;
-     destruct (X.compare x' x); auto; absurd (X.lt x' x); eauto.
+    apply Lt; unfold lt; simpl; MapS.Raw.MX.compare; right; auto.
+    apply Eq; unfold eq; simpl; MapS.Raw.MX.compare; auto.
+    apply Gt; unfold lt; simpl; MapS.Raw.MX.compare; auto.
+    apply Gt; unfold lt; simpl; MapS.Raw.MX.compare; auto.
+    apply Gt; unfold lt; simpl; MapS.Raw.MX.compare; auto.
     Qed.
 
 End Make_ord. 
